src/simple-proof/proof-ec/OperationalSemantics.v
@@ -1,0 +1,308 @@
+Set Implicit Arguments.
+
+Require Import Coq.Program.Equality.
+Require Import LibLN.
+Require Import Definitions Binding.
+
+(** * Normal Forms
+A normal form is defined in the WadlerFest DOT paper as:
+
+[n ::= x | v | let x = v in n]
+
+This corresponds to an evaluation context of the form
+[(let x = v in)* [ ]] whose hole is filled by a variable [x]
+or value [v]. *)
+
+Inductive normal_form: trm -> Prop :=
+| nf_var: forall x, normal_form (trm_var x)
+| nf_val: forall v, normal_form (trm_val v)
+| nf_let: forall v t, normal_form t -> normal_form (trm_let (trm_val v) t).
+
+(** * Operational Semantics
+
+The first four reduction rules correspond directly to the rules in Figure 7 of the paper.
+
+The last two rules are congruence rules that implement the meaning of evaluation contexts.
+Specifically, if a term [u] decomposes into an evaluation context and subterm
+as [u = e[t]] and [e[t]] reduces to [e[t']] according to the rules from Figure 7,
+then the purpose of the two congruence rules is to ensure that [u] also reduces
+to [u'], where [u'] is the term [u' = e[t']]. The grammar for evaluation contexts
+in the paper is:
+
+[e ::= [] | let x = [] in t | let x = v in e]
+
+A sentential form [eta] in a derivation of an evaluation context [e] is a string
+of terminals (the elements of DOT terms) and the non-terminal [e]. Define
+[e(eta)] to be a string of terminals formed by replacing [e] with [[]] in [eta].
+We argue that whenever [eta_1] directly derives [eta_2] ([eta_1 => eta_2]),
+and the reduction rules infer that [e(eta_2)[t_2] |-> e(eta_2)[t_2']], then the
+reduction rules also infer that [e(eta_1)[t_1] |-> e(eta_1)[t_1']], where
+[e(eta_2)[t_2] = e(eta_1)[t_1]] and [e(eta_2)[t_2'] = e(eta_1)[t_1']].
+The argument is by considering each of the three cases
+in the evaluation context grammar that justify [eta_1 => eta_2].
+The first case replaces [e] with [[]], so [e(eta_1) = e(eta_2)], so the conclusion
+trivially holds. The second case replaces [e] with [let x = [] in t]. In this case,
+the reduction congruence rule [red_let_trm] has [e(eta_2)[t_2] |-> e(eta_2)[t_2']]
+as a premise and [e(eta_1)[t_1] |-> e(eta_1)[t_1']] as a conclusion. The third case
+replaces [e] with [let x = v in e].  Similarly, the congruence rule [red_let_val]
+has [e(eta_2)[t_2] |-> e(eta_2)[t_2']] as a premise and [e(eta_1)[t_1] |-> e(eta_1)[t_1']]
+as a conclusion. Thus, whenever [eta_1 => eta_2] and [e(eta_2)[t_2] |-> e(eta_2)[t_2']],
+we also have that [e(eta_1)[t_1] |-> e(eta_1)[t_1']].
+
+Reasoning inductively about the steps in the context-free grammar derivation of [e],
+for every sentential
+form [eta] that occurs in that derivation, the congruence reduction rules infer that
+[e(eta)[u] |-> e(eta)[u']], where
+[e(eta)[u] = e[t]] and [e(eta)[u'] = e[t']]. In particular, this is true for the
+sentential form [eta = e], the first sentential form of every derivation. Since
+[e(eta) = e(e) = []], we have shown that the congruence reduction rules infer that [u |-> u'].
+
+Starting with an evaluation context [e] in its conclusion, the [red_let_val] rule appends
+[let x = v] to the context to yield a new context used in its premise.
+(More precisely, the rule replaces the non-terminal [e] within the context in the conclusion by
+[let x = v in e].) This is the only reduction rule that modifies an existing evaluation context. Therefore,
+in a derivation of a reduction judgment [u |-> u'] in an empty evaluation context, every evaluation context
+that appears in the derivation is of the form [let x_1 = v_1 in ... let x_n = v_n in []].
+Therefore, in order to be able to represent every step of every such derivation of a reduction
+judgement in the Coq proof, it is sufficient to represent evaluation contexts by a data structure
+that can represent all evaluation contexts of this form. The proof represents these evaluation
+contexts by a list of pairs of variables and values.
+*)
+
+
+Reserved Notation "e '[' t1 '|->' t2 ']'" (at level 60, t1 at level 39).
+
+Inductive red : ec -> trm -> trm -> Prop :=
+(** [e(x) = lambda(T)t]    #<br>#
+    [――――――――――――――――――――]  #<br>#
+    [e[x y] |-> e[t^y] ]  *)
+| red_apply : forall x y e T t,
+    lc_trm (trm_app (avar_f x) (avar_f y)) ->
+    binds x (val_lambda T t) e ->
+    e [ trm_app (avar_f x) (avar_f y) |-> open_trm y t ]
+(** [e(x) = nu(T)...{a = t}...]  #<br>#
+    [―――――――――――――――――――――――――]  #<br>#
+    [e[x.a] |-> e[t]]  *)
+| red_project : forall x a e T ds t,
+    lc_trm (trm_sel (avar_f x) a) ->
+    binds x (val_new T ds) e ->
+    defs_has (open_defs x ds) (def_trm a t) ->
+    e [ trm_sel (avar_f x) a |-> t ]
+(** [e[let x = y in t] |-> e[t^y]] *)
+| red_let_var : forall y t e,
+    lc_trm (trm_let (trm_var (avar_f y)) t) ->
+    e [ trm_let (trm_var (avar_f y)) t |-> open_trm y t ]
+(** [e[let x = (let y = s in t) in u] |-> e[let y = s in let x = t in u]] *)
+| red_let_let : forall s t u e,
+    lc_trm (trm_let (trm_let s t) u) ->
+    e [ trm_let (trm_let s t) u |-> trm_let s (trm_let t u) ]
+(** [e[t] |-> e[t']]                            #<br>#
+    [――――――――――――――――――――――――――――――――――――――――]  #<br>#
+    [e[let x = t in u] |-> e[let x = t' in u]]     *)
+| red_let_trm : forall e t t' u,
+    lc_trm (trm_let t u) ->
+    e [ t |-> t' ] ->
+    e [ trm_let t u |-> trm_let t' u ]
+(** [(e, x = v) [t] |-> (e, x = v) [t']]        #<br>#
+    [――――――――――――――――――――――――――――――――――――――――]   #<br>#
+    [e[let x = v in t] |-> e[let x = v in t']]   *)
+| red_let_val: forall e t t' v L,
+    lc_trm (trm_let (trm_val v) t) ->
+    (forall x, x \notin L  ->
+      (e & x ~ v) [ open_trm x t |-> open_trm x t' ]) ->
+    e [ trm_let (trm_val v) t |-> trm_let (trm_val v) t' ]
+where "e [ t |-> t' ]" := (red e t t').
+Hint Constructors red normal_form.
+
+(** Reduction in an empty context *)
+Notation "t '|->' u" := (empty [t |-> u]) (at level 50).
+
+(** Typing in an empty context *)
+Notation "'⊢' t ':' T" := (empty ⊢ t: T) (at level 40, t at level 59).
+
+(** If [e] is locally closed and [e[t] |-> e[t']], then [t'] is locally closed.  *)
+Lemma lc_env_eval_to_lc_trm : forall e t t',
+    lc_ec e ->
+    e [t |-> t'] ->
+    lc_trm t'.
+Proof with auto.
+  introv Hlce He.
+  induction He;
+    match goal with
+    | [ H : lc_at_trm _ _ |- _ ] => inversions H
+    end;
+    repeat constructor;
+    do 2 try
+       match goal with
+       | [ H : binds _ _ _ |- _ ] => apply lc_ec_binds_inv in H; eauto
+       | [ H : lc_at_val _ _ |- _ ] => inversions H
+       | [ H : lc_at_trm _ _ |- _ ] => solve [inversions H; auto]
+       end;
+    try applys lc_at_to_open_trm_val_def_defs;
+    eauto.
+  - apply lc_defs_has in H1... inversion H1...
+    applys lc_at_to_open_trm_val_def_defs...
+  - eapply lc_at_relaxing_trm_val_def_defs; try eassumption.
+    omega.
+  - inversion H4. pick_fresh x.
+    assert (x \notin L); auto.
+    assert (lc_ec (e & x ~ v)); auto.
+    specialize (H1 x H3 H6).
+    applys open_to_lc_at_trm_val_def_defs. eassumption.
+Qed.
+
+(** The next two lemmas show that if [t^x] is in normal form, then [t] is in normal form. *)
+Lemma open_rec_preserve_normal_form: forall k x t,
+    x \notin fv_trm t ->
+    normal_form (open_rec_trm k x t) ->
+    normal_form t.
+Proof.
+  intros. generalize dependent x.
+  generalize dependent k.
+  induction t; auto; intros;
+    try solve [
+    unfold open_trm in H0; unfold open_rec_trm in H0;
+    inversion H0].
+  unfold open_trm in H0. unfold open_rec_trm in H0.
+  inversion H0. fold open_rec_trm in *.
+  unfold fv_trm in H. fold fv_trm in H.
+  assert (x \notin fv_trm t2); auto.
+  specialize (IHt2 _ _ H4 H2).
+
+  destruct t1; simpl; inversion H1.
+  constructor. auto.
+Qed.
+
+(** See previous lemma [open_rec_preserve_normal_form]. *)
+Lemma open_preserve_normal_form : forall x t,
+    x \notin fv_trm t ->
+    normal_form (open_trm x t) ->
+    normal_form t.
+Proof.
+  apply open_rec_preserve_normal_form.
+Qed.
+
+(** [x] fresh                            #<br>#
+    [e] and [v] are locally closed       #<br>#
+    [(e, x=v)[t^x] |-> (e, x=v)[t']]     #<br>#
+    [――――――――――――――――――――――――――――――――――] #<br>#
+    [exists f. x \notin fv(f) and t' = f^x    *)
+Lemma open_rec_eval_to_open_rec : forall e x t t' v,
+    x \notin dom e \u fv_trm t \u fv_val v ->
+    lc_ec e -> lc_val v ->
+    e & x ~ v[ open_trm x t |-> t'] ->
+    exists f, (x \notin (fv_trm f)) /\ t' = open_trm x f.
+Proof.
+  intros. exists (close_trm x t'). remember (close_trm x t') as ct. split.
+  - subst ct. apply close_rec_trm_val_def_defs_no_capture.
+  - symmetry. rewrite Heqct. apply open_left_inverse_close_trm_val_def_defs.
+    eauto using lc_env_eval_to_lc_trm, lc_ec_cons.
+Qed.
+
+(** Substitution for reduction *)
+
+(** [x, y] fresh                                                  #<br>#
+    [(e1, x=v, e2)[t1] |-> (e1, x=v, e2)[t2]]                     #<br>#
+    [―――――――――――――――――――――――――――――――――――――――――――――――――――――――――――] #<br>#
+    [(e1, y=v[y/x], e2)[t1[y/x]] |-> (e1, y=v[y/x], e2)[t2[y/x]]] *)
+Lemma eval_renaming_subst : forall x y e1 e2 v t1 t2,
+    x \notin dom e1 \u fv_ec_vals e1 \u dom e2 ->
+    y \notin dom e1 \u fv_ec_vals e1
+      \u dom e2 \u fv_ec_vals e2 \u fv_val v \u fv_trm t1 ->
+    (e1 & x ~ v & e2)[t1 |-> t2] ->
+    (e1 & y ~ subst_val x y v & subst_env x y e2)[subst_trm x y t1 |-> subst_trm x y t2].
+Proof.
+  Local Hint Resolve binds_subst_env.
+
+  Local Ltac contra_bind :=
+    repeat match goal with
+           | [ H : _ \notin _ \u _ |- _ ] => apply notin_union in H; destruct H
+           end;
+    match goal with
+    | [ _ : ?x \notin dom ?e, _ : binds ?x _ ?e |- _ ] =>
+      exfalso; eapply binds_fresh_inv; [eassumption | auto 1]
+    end.
+
+  Local Ltac solve_left_most :=
+    apply binds_concat_left; unfold subst_env; try rewrite dom_map;
+    try rewrite (proj1 (proj2 (subst_fresh_trm_val_def_defs _ _))); auto;
+    eapply binds_fv_ec_vals; eauto 2.
+
+  introv Hfx Hfy He. dependent induction He; simpls.
+  - apply binds_middle_inv in H0; destruct_all; case_if; subst;
+      try contra_bind;
+      rewrite subst_open_commut_trm; unfold subst_fvar; case_if;
+        apply red_apply with (subst_typ x y T);
+          assert (Hs : val_lambda (subst_typ x y T) (subst_trm x y t) =
+                       subst_val x y (val_lambda T t)) by auto;
+          auto 2;
+          rewrite Hs;
+          try match goal with
+              | [ |- binds ?y _ (_ & ?y ~ _ & _) ] =>
+                apply binds_middle_eq; unfold subst_env; rewrite dom_map; auto 1
+              end;
+          try solve [apply binds_concat_right, binds_subst_env; trivial];
+          solve_left_most.
+  - apply binds_middle_inv in H0; destruct_all; case_if; subst;
+      try contra_bind;
+      apply red_project with (T:=subst_typ x y T) (ds:=subst_defs x y ds); auto 1;
+        assert (Hs : val_new (subst_typ x y T) (subst_defs x y ds) = subst_val x y (val_new T ds));
+        auto 2;
+        try rewrite Hs.
+    + apply binds_concat_right; apply binds_subst_env; trivial.
+    + apply open_subst_defs; auto.
+    + apply binds_middle_eq; unfold subst_env; rewrite dom_map; auto.
+    + apply open_subst_defs2; auto.
+    + solve_left_most.
+    + apply open_subst_defs; auto.
+  - case_if; simpls;
+      subst; rewrite subst_open_commut_trm; unfold subst_fvar;
+        case_if; constructor;
+          inversion H; constructor; auto;
+            apply lc_at_subst_trm_val_def_defs; trivial.
+  - inversion H. inversion H2.
+    repeat constructor; auto;
+      apply lc_at_subst_trm_val_def_defs; trivial.
+  - inversion H.
+    repeat constructor; auto;
+      apply lc_at_subst_trm_val_def_defs; trivial.
+  - econstructor.
+    + inversion H. inversion H4.
+      repeat constructor;
+        apply lc_at_subst_trm_val_def_defs; trivial.
+    + intros.
+      instantiate (1 := L \u dom e1 \u fv_ec_vals e1 \u dom e2 \u fv_ec_vals e2
+                            \u fv_val v \u fv_val v0 \u fv_trm t \u \{x} \u \{y}) in H2.
+
+      assert (x0 <> x) by auto.
+      assert (x0 <> y) by auto.
+
+      assert (subst_fvar x y x0 = x0). {
+        unfold subst_fvar. case_if; auto.
+      }
+      rewrite <- H5.
+      rewrite <- subst_open_commut_trm. rewrite <- subst_open_commut_trm.
+      rewrite H5.
+
+      assert (x0 \notin L) by auto.
+      specialize (H1 _ H6 v (e2 & x0 ~ v0) e1).
+
+      assert (y \notin fv_trm (open_trm x0 t)). {
+        apply open_fv_trm_val_def_defs; auto.
+      }
+      assert (y \notin fv_ec_vals (e2 & x0 ~ v0)) by rewrite~ fv_ec_vals_push_eq.
+
+      assert (y \notin dom e1 \u fv_ec_vals e1
+                \u dom (e2 & x0 ~ v0) \u fv_ec_vals (e2 & x0 ~ v0)
+                \u fv_val v \u fv_trm (open_trm x0 t)); auto.
+
+      assert (x \notin dom e1 \u fv_ec_vals e1 \u dom (e2 & x0 ~ v0)); auto.
+
+      assert (subst_env x y (e2 & x0 ~ v0) = subst_env x y e2 & x0 ~ subst_val x y v0). {
+        unfold subst_env. apply map_push.
+      }
+      specialize (H1 H9 _ H10).
+      rewrite H11 in H1.
+      rewrite? concat_assoc in H1.
+      apply H1. auto.
+Qed.
