src/simple-proof/proof-ec/Safety.v
@@ -1,0 +1,309 @@
+(** printing ⊢#    %\vdash_{\#}%    #&vdash;<sub>&#35;</sub>#     *)
+(** printing ⊢##   %\vdash_{\#\#}%  #&vdash;<sub>&#35&#35</sub>#  *)
+(** printing ⊢##v  %\vdash_{\#\#v}% #&vdash;<sub>&#35&#35v</sub># *)
+(** printing ⊢!    %\vdash_!%       #&vdash;<sub>!</sub>#         *)
+(** remove printing ~ *)
+
+Set Implicit Arguments.
+
+Require Import Coq.Program.Equality.
+Require Import LibLN.
+Require Import Definitions.
+Require Import RecordAndInertTypes.
+Require Import Binding.
+Require Import OperationalSemantics.
+Require Import Weakening SubEnvironments Narrowing PreciseTypes Substitution CanonicalForms.
+
+(** * Progress *)
+
+(** If a value [v] has type [T], then [v] has a precise type [T']
+    that is a subtype of [T].
+    This lemma corresponds to Lemma 3.15 in the paper. *)
+Lemma val_typing: forall G v T,
+  G ⊢ trm_val v : T ->
+  exists T', G ⊢! trm_val v : T' /\
+        G ⊢ T' <: T.
+Proof.
+  intros G v T H. dependent induction H; eauto.
+  destruct (IHty_trm _ eq_refl) as [T' [Hty Hsub]]. eauto.
+Qed.
+
+(** [e] and [t] are locally closed          #<br>#
+    [G' ⪯ G]                                #<br>#
+    inert [G']                              #<br>#
+    [e: G']                                 #<br>#
+    [G ⊢ t: T]                              #<br>#
+    [―――――――――――――――――――――――――――――]         #<br>#
+    [t] is in normal form or [e[t] |-> e[t']] *)
+Lemma progress_ec: forall G' G e t T,
+    lc_ec e ->
+    lc_trm t ->
+    G' ⪯ G ->
+    inert G' ->
+    well_typed G' e ->
+    G ⊢ t: T ->
+    ok G ->
+    (normal_form t \/ exists t', e[t |-> t']).
+Proof with auto.
+  introv Hlce Hlc Hsenv Hig Hwt Ht Hokg. gen G' e.
+  induction Ht; eauto; intros.
+  - Case "ty_all_elim".
+    apply narrow_typing with (G':=G') in Ht1; auto.
+    destruct (canonical_forms_fun Hig Hwt Ht1) as [L [T' [t [Bis [Hsub Hty]]]]].
+    right. repeat eexists. apply* red_apply.
+  - Case "ty_new_elim".
+    apply narrow_typing with (G':=G') in Ht; auto.
+    destruct (canonical_forms_obj Hig Hwt Ht) as [S [ds [t [Bis [Has Ty]]]]].
+    right. repeat eexists. apply* red_project.
+  - Case "ty_let".
+    destruct t.
+    + SCase "t = trm_var a".
+      apply narrow_typing with (G':=G') in Ht; auto.
+      right.
+      assert (var_typing_implies_avar_f: forall G a T, G ⊢ trm_var a : T -> exists x, a = avar_f x)
+        by (introv HGat; dependent induction HGat; eauto).
+      destruct (var_typing_implies_avar_f _ _ _ Ht); subst.
+      exists (open_trm x u). constructor...
+    + SCase "t = trm_val v".
+      apply val_typing in Ht.
+      destruct Ht as [T' [H1 H2]].
+      pose proof (precise_inert_typ H1) as Hpit.
+      pick_fresh x.
+      destruct H0 with (x:=x) (G' := G' & x ~ T') (e := e & x ~ v); auto 2.
+      * inversion Hlc. trivial. apply lc_at_to_open_trm_val_def_defs...
+      * intros. eapply subenv_trans; econstructor; eauto.
+      * constructor; auto. inversion Hlc. inversion H5. trivial.
+      * intros. apply precise_to_general in H1.
+        constructor; auto. eapply narrow_typing in H1; eauto.
+      * left.
+        destruct u; auto; apply open_preserve_normal_form in H3; auto.
+      * right. destruct H3.
+        pose proof H3. inversion Hlc. inversion H7.
+        apply open_rec_eval_to_open_rec in H3; auto.
+        destruct_all. subst.
+        exists (trm_let (trm_val v) x1).
+
+        apply red_let_val with (L \u dom G \u fv_ctx_types G \u dom G
+                                  \u fv_ctx_types G \u dom e \u fv_ec_vals e
+                                  \u fv_trm (open_trm x u) \u fv_val v \u fv_typ T
+                                  \u fv_typ U \u fv_typ T' \u fv_trm x1
+                                  \u dom (empty : ec) \u fv_ec_vals empty); auto.
+        intros.
+
+        replace (e & x ~ v) with (e & x ~ v & empty) in H4;
+          try (rewrite <- concat_empty_r; trivial).
+
+
+        replace (e & x0 ~ v) with (e & x0 ~ v & empty);
+        try (rewrite <- concat_empty_r; trivial).
+
+        assert (Hsubstv : subst_val x x0 v = v). {
+          apply subst_fresh_trm_val_def_defs. auto.
+        }
+        rewrite <- Hsubstv.
+
+        assert (Hleft : open_trm x0 u = subst_trm x x0 (open_trm x u)). {
+          apply subst_intro_trm. auto.
+        }
+        rewrite Hleft.
+
+        assert (Hright : open_trm x0 x1 = subst_trm x x0 (open_trm x x1)). {
+          apply subst_intro_trm. auto.
+        }
+        rewrite Hright.
+
+        replace empty with (subst_env x x0 empty); try apply map_empty; trivial.
+
+        apply eval_renaming_subst; auto.
+    + SCase "t = trm_sel a t".
+      right.
+      inversion Hlc.
+      destruct (IHHt H3 Hokg G' Hsenv Hig e Hlce Hwt) as [Hnf | [t' Hr]]. inversion Hnf.
+      eexists. constructor*.
+    + SCase "t = trm_app a a0".
+      right.
+      inversion Hlc.
+      destruct (IHHt H3 Hokg G' Hsenv Hig e Hlce Hwt) as [Hnf | [t' Hr]]. inversion Hnf.
+      eexists. constructor*.
+    + SCase "t = trm_let t1 t2".
+      right. eexists. constructor. inversion Hlc. trivial.
+Qed.
+
+(** ** Progress Theorem
+    If [⊢ t : T], then either [t] is a normal form,
+    or [t]] reduces to some [t']. *)
+Theorem progress: forall t T,
+    lc_trm t ->
+    ⊢ t: T ->
+    normal_form t \/ (exists t', t |-> t').
+Proof.
+  intros. apply* progress_ec.
+Qed.
+
+(** * Preservation *)
+
+(** [t] is locally closed   #<br>#
+    [G' ⪯ G]                #<br>#
+    [e: G']                 #<br>#
+    inert [G']              #<br>#
+    [G ⊢ t: T]              #<br>#
+    [e[t] |-> e[t']]        #<br>#
+    [ok G]                  #<br>#
+    [―――――――――――――――――――]   #<br>#
+    [G' ⊢ t': T]            *)
+Lemma preservation_ec: forall G G' e t t' T,
+    lc_trm t ->
+    G' ⪯ G ->
+    well_typed G' e ->
+    inert G' ->
+    G ⊢ t: T ->
+    e[t |-> t'] ->
+    ok G ->
+    G' ⊢ t': T.
+Proof.
+  Local Hint Resolve open_bound_lc_trm.
+  introv Hlc Hsenv Hwt Hi Ht Hr Hok. gen e t'. gen G'.
+  induction Ht; introv Hsenv Hi Hwt Hr; try solve [inversions Hr].
+  - Case "ty_all_elim".
+    apply narrow_typing with (G':=G') in Ht1; auto.
+    destruct (canonical_forms_fun Hi Hwt Ht1) as [L [T' [t [Bis [Hsub Hty]]]]].
+    inversions Hr.
+    apply (binds_func H4) in Bis. inversions Bis.
+    pick_fresh y. apply~ renaming_typ.
+    apply (narrow_typing Ht2); auto.
+  - Case "ty_new_elim".
+    apply narrow_typing with (G':=G') in Ht; auto.
+    destruct (canonical_forms_obj Hi Hwt Ht) as [S [ds [t [Bis [Has Ty]]]]].
+    inversions Hr.
+    apply (binds_func H3) in Bis. inversions Bis.
+    rewrite <- (defs_has_inv Has H5). assumption.
+  - Case "ty_let".
+    inversions Hr.
+    * SCase "red_let_var".
+      pick_fresh x. assert (x \notin L); auto. specialize (H x H1).
+      apply subst_ty_trm with (y:=y) in H; auto.
+      -- assert (subst_typ x y U = U). {
+           apply subst_fresh_typ_dec. auto.
+         }
+         rewrite H2 in H.
+         assert (open_trm y u = subst_trm x y (open_trm x u)). {
+           apply subst_intro_trm. auto.
+         }
+         rewrite <- H3 in H.
+         apply narrow_typing with (G':=G') in H; auto.
+      -- assert (subst_typ x y T = T). {
+           apply subst_fresh_typ_dec. auto.
+         }
+         rewrite H2. trivial.
+    * SCase "red_let_let".
+      clear H0 IHHt.
+      assert (forall x, x \notin (L \u dom G) -> G & x ~ T ⊢ open_trm x u : U). {
+        intros. assert (x \notin L); auto.
+      }
+      clear H.
+      dependent induction Ht.
+      -- apply narrow_typing with (G' := G') in Ht; eauto.
+         remember ((((((((((((L \u L0) \u dom G) \u fv_ctx_types G) \u dom G')
+                            \u fv_ctx_types G') \u dom e) \u fv_trm u) \u fv_trm s)
+                        \u fv_trm t0) \u fv_typ U) \u fv_typ T) \u fv_typ U0) as bigL.
+         econstructor; eauto. intros.
+         instantiate (1 := bigL) in H2.
+         unfold open_trm, open_rec_trm. fold open_rec_trm.
+
+         assert (open_rec_trm 1 x u = u). {
+           inversion H5. apply open_bound_lc_trm.
+           apply lc_at_to_open_trm_val_def_defs. trivial.
+         }
+         rewrite H3. clear H3.
+
+         rewrite HeqbigL in H2.
+         assert (x \notin L0); auto.
+         specialize (H _ H3).
+         assert (G' & x ~ T ⪯ G & x ~ T); auto.
+         apply narrow_typing with (G' := G' & x ~ T) in H; auto.
+         rewrite <- HeqbigL in H2.
+         econstructor; eauto.
+         intros. instantiate (1 := bigL \u \{ x }) in H6.
+         subst bigL.
+         assert (x0 \notin L \u dom G); auto.
+         specialize (H1 _ H7).
+         assert (G' & x0 ~ U0 ⊢ open_trm x0 u : U). {
+           eapply narrow_typing; [eassumption |]; auto.
+         }
+         eapply (proj1 weaken_rules); eauto.
+      -- eapply IHHt; eauto; intros.
+         specialize (H0 _ H1).
+         eapply narrow_typing; eauto.
+    * SCase "red_let_trm".
+      inversion Hlc.
+      specialize (IHHt H3 Hok _ Hsenv Hi _ Hwt t'0 H6).
+      eapply ty_let; eauto. intros.
+      instantiate (1 := (((((((((L \u dom G) \u fv_ctx_types G) \u dom G')
+                                \u fv_ctx_types G') \u dom e) \u fv_trm t) \u fv_trm u)
+                            \u fv_trm t'0) \u fv_typ T) \u fv_typ U) in H7.
+      assert (x \notin L); auto.
+      specialize (H _ H8).
+      apply (narrow_typing H); auto.
+    * SCase "red_let_val".
+      apply val_typing in Ht.
+      destruct Ht as [T' [H1 H2]].
+      pose proof (precise_inert_typ H1) as Hpit.
+      pose proof H1 as Htt.
+      apply precise_to_general in Htt.
+      apply narrow_typing with (G':=G') in Htt; auto.
+      pick_fresh x. assert (x \notin L); auto.
+      assert (ok (G & x ~ T)); auto.
+      assert (G' & x ~ T' ⪯ G & x ~ T). {
+        apply subenv_trans with (G & x ~ T'); auto.
+      }
+      assert (inert (G' & x ~ T')) by auto.
+      assert (well_typed (G' & x ~ T') (e & x ~ v)) by auto.
+      assert (x \notin L0) by auto.
+      inversion Hlc.
+
+      apply (proj1 (lc_at_to_open_trm_val_def_defs x)) in H14.
+      specialize (H0 _ H3 H14 H5 (G' & x ~ T') H7 H8 (e & x ~ v) H9 _ (H6 _ H10)).
+      apply_fresh ty_let as y; eauto.
+
+      apply weaken_ty_trm with (G2:=(y ~ T')) in H0; auto.
+
+      pose proof (proj1 (subst_rules y T')) as Hsubst.
+      specialize (Hsubst _ _ _ H0 G' (y ~ T') x).
+      assert (HsubstU : subst_typ x y U = U). {
+        apply subst_fresh_typ. auto.
+      }
+
+      assert (Hxyt : subst_typ x y T' = T'). {
+        apply subst_fresh_typ. auto.
+      }
+
+      assert (Hopeny : subst_ctx x y (y ~ T') = y ~ T'). {
+        unfold subst_ctx. rewrite map_single, Hxyt. trivial.
+      }
+
+      assert (Hopent : subst_trm x y (open_trm x t'0) = open_trm y t'0). {
+        rewrite subst_open_commut_trm.
+        rewrite (proj1 (subst_fresh_trm_val_def_defs _ _)); auto.
+        unfold subst_fvar. case_if; auto.
+      }
+      rewrite HsubstU, Hopeny, Hopent in Hsubst.
+
+      apply Hsubst; auto.
+      rewrite Hxyt; auto.
+
+  - apply narrow_typing with (G' := G') in Ht; auto.
+    apply narrow_subtyping with (G' := G') in H; auto.
+    eauto.
+Qed.
+
+
+(** ** Preservation Theorem
+    If [⊢ t : T] and [t |-> t'], then [⊢ t': T]. *)
+Theorem preservation: forall (t t' : trm) T,
+    lc_trm t ->
+    ⊢ t: T ->
+    t |-> t' ->
+    ⊢ t' : T.
+Proof.
+  intros. eapply preservation_ec; eauto.
+Qed.
